<?xml version="1.0" encoding="utf-8"?>
<rdf:RDF
  xmlns:rdfs="http://www.w3.org/2000/01/rdf-schema#"
  xmlns:owl="http://www.w3.org/2002/07/owl#"
  xmlns:rdf="http://www.w3.org/1999/02/22-rdf-syntax-ns#"
>
  <owl:Class rdf:about="#Baías">
    <rdfs:label>Baías</rdfs:label>
    <rdfs:comment>These are bodies of water partially enclosed by land but with a wide mouth, providing shelter to various marine species.</rdfs:comment>
    <rdfs:subClassOf rdf:resource="#ecossistemas%20costeiros%20brasileiros"/>
  </owl:Class>
  <owl:Class rdf:about="#Fauna%20arenosa">
    <rdfs:label>Fauna arenosa</rdfs:label>
    <rdfs:comment>In "fauna de praia" is a subcategory of Fauna de praia. This refers to the animal life that inhabits sandy beaches.</rdfs:comment>
    <rdfs:subClassOf rdf:resource="#Fauna%20de%20praia"/>
  </owl:Class>
  <owl:Class rdf:about="#Recifes%20de%20coral%20tubulares">
    <rdfs:label>Recifes de coral tubulares</rdfs:label>
    <rdfs:comment>These are a type of coral known for their tube-like structure.</rdfs:comment>
    <rdfs:subClassOf rdf:resource="#Zonas%20de%20recifes%20de%20plataforma"/>
    <rdfs:subClassOf rdf:resource="#Colônias%20de%20corais"/>
  </owl:Class>
  <owl:Class rdf:about="#Tubarões%20e%20raias%20de%20recifes%20de%20coral">
    <rdfs:label>Tubarões e raias de recifes de coral</rdfs:label>
    <rdfs:comment>These are sharks and rays that inhabit or visit coral reefs, often as top predators.</rdfs:comment>
    <rdfs:subClassOf rdf:resource="#Recifes%20de%20coral%20de%20plataforma%20continental"/>
    <rdfs:subClassOf rdf:resource="#Recifes%20de%20coral%20de%20franja"/>
    <rdfs:subClassOf rdf:resource="#Zonas%20de%20recifes%20de%20barreira"/>
    <rdfs:subClassOf rdf:resource="#Zonas%20de%20frente%20de%20recife"/>
  </owl:Class>
  <owl:Class rdf:about="#Corais%20massivos">
    <rdfs:label>Corais massivos</rdfs:label>
    <rdfs:comment>These are hard corals that form massive, dome-shaped colonies.</rdfs:comment>
    <rdfs:subClassOf rdf:resource="#Corais%20construtores%20de%20recifes"/>
  </owl:Class>
  <owl:Class rdf:about="#Zonas%20mortas%20do%20recife%20de%20coral">
    <rdfs:label>Zonas mortas do recife de coral</rdfs:label>
    <rdfs:comment>These are areas of the reef where coral growth has ceased, often due to environmental stress or damage.</rdfs:comment>
    <rdfs:subClassOf rdf:resource="#Zonas%20de%20recifes%20de%20barreira"/>
    <rdfs:subClassOf rdf:resource="#Coral%20reef%20zones%20(fore%20reef"/>
  </owl:Class>
  <owl:Class rdf:about="#Zonas%20de%20transição">
    <rdfs:label>Zonas de transição</rdfs:label>
    <rdfs:comment>These are areas within an estuary where saltwater from the sea mixes with freshwater from rivers, creating a unique environment that supports a diverse range of species.</rdfs:comment>
    <rdfs:subClassOf rdf:resource="#Estuários"/>
  </owl:Class>
  <owl:Class rdf:about="#Lagoas%20costeiras">
    <rdfs:label>Lagoas costeiras</rdfs:label>
    <rdfs:comment>These are coastal lagoons, which are shallow bodies of water separated from the sea by a barrier.</rdfs:comment>
    <rdfs:subClassOf rdf:resource="#ecossistemas%20costeiros%20brasileiros"/>
  </owl:Class>
  <owl:Class rdf:about="#Praias%20de%20barra">
    <rdfs:label>Praias de barra</rdfs:label>
    <rdfs:comment>These are beaches characterized by the presence of a sandbar, a landform made of sand that has been deposited by the sea.</rdfs:comment>
    <rdfs:subClassOf rdf:resource="#Praias%20arenosas"/>
  </owl:Class>
  <owl:Class rdf:about='#Corais%20do%20tipo%20"elkhorn"'>
    <rdfs:label>Corais do tipo "elkhorn"</rdfs:label>
    <rdfs:comment>These are corals that have branching structures that resemble elk antlers.</rdfs:comment>
    <rdfs:subClassOf rdf:resource="#Corais%20construtores%20de%20recifes"/>
  </owl:Class>
  <owl:Class rdf:about="#Zonas%20de%20maré%20baixa">
    <rdfs:label>Zonas de maré baixa</rdfs:label>
    <rdfs:comment>These are areas within an estuary that are exposed at low tide.</rdfs:comment>
    <rdfs:subClassOf rdf:resource="#Estuários"/>
  </owl:Class>
  <owl:Class rdf:about="#Recifes%20de%20coral%20isolados">
    <rdfs:label>Recifes de coral isolados</rdfs:label>
    <rdfs:comment>These are similar to Recifes de patch, small and isolated reefs growing from the open bottom.</rdfs:comment>
    <rdfs:subClassOf rdf:resource="#Zonas%20de%20recifes%20de%20coral"/>
  </owl:Class>
  <owl:Class rdf:about="#Corais%20duros">
    <rdfs:label>Corais duros</rdfs:label>
    <rdfs:comment>These are species of hard corals.</rdfs:comment>
    <rdfs:subClassOf rdf:resource="#Corais%20construtores%20de%20recifes"/>
    <rdfs:subClassOf rdf:resource="#Recifes%20de%20coral%20de%20franja"/>
    <rdfs:subClassOf rdf:resource="#Zonas%20de%20lagoa%20de%20recife"/>
  </owl:Class>
  <owl:Class rdf:about="#Manguezais">
    <rdfs:label>Manguezais</rdfs:label>
    <rdfs:comment>These are coastal wetlands found in tropical and subtropical regions, characterized by halophytic (salt loving) trees, shrubs and other plants growing in brackish to saline tidal waters.</rdfs:comment>
    <rdfs:subClassOf rdf:resource="#ecossistemas%20costeiros%20brasileiros"/>
  </owl:Class>
  <owl:Class rdf:about="#Costões%20rochosos">
    <rdfs:label>Costões rochosos</rdfs:label>
    <rdfs:comment>These are rocky coastal areas that are constantly eroded by the action of the sea.</rdfs:comment>
    <rdfs:subClassOf rdf:resource="#ecossistemas%20costeiros%20brasileiros"/>
  </owl:Class>
  <owl:Ontology rdf:about="file:///ecossistemas_costeiros_brasileiros.owl"/>
  <owl:Class rdf:about="#Zonas%20de%20recifes%20de%20plataforma">
    <rdfs:label>Zonas de recifes de plataforma</rdfs:label>
    <rdfs:comment>These are areas within a platform reef where coral reefs are found.</rdfs:comment>
    <rdfs:subClassOf rdf:resource="#Zonas%20de%20recifes%20de%20coral"/>
  </owl:Class>
  <owl:Class rdf:about="#Corais%20construtores%20de%20recifes">
    <rdfs:label>Corais construtores de recifes</rdfs:label>
    <rdfs:comment>These are species of corals that produce calcium carbonate, forming the structural framework of coral reefs.</rdfs:comment>
    <rdfs:subClassOf rdf:resource="#Biodiversidade%20de%20recifes%20de%20corais"/>
  </owl:Class>
  <owl:Class rdf:about="#Fauna%20de%20praia">
    <rdfs:label>Fauna de praia</rdfs:label>
    <rdfs:comment>This refers to the animal life that inhabits sandy beaches.</rdfs:comment>
    <rdfs:subClassOf rdf:resource="#Praias%20arenosas%20com%20restingas"/>
  </owl:Class>
  <owl:Class rdf:about="#Praias%20arenosas">
    <rdfs:label>Praias arenosas</rdfs:label>
    <rdfs:comment>These are sandy beaches, which are loose deposits of sand, gravel or pebble covering the shoreline.</rdfs:comment>
    <rdfs:subClassOf rdf:resource="#ecossistemas%20costeiros%20brasileiros"/>
  </owl:Class>
  <owl:Class rdf:about="#Praias%20arenosas%20com%20restingas">
    <rdfs:label>Praias arenosas com restingas</rdfs:label>
    <rdfs:comment>These are beaches that are associated with restingas, a type of coastal vegetation found on sandy, nutrient-poor soils.</rdfs:comment>
    <rdfs:subClassOf rdf:resource="#Praias%20arenosas"/>
  </owl:Class>
  <owl:Class rdf:about="#Zonas%20de%20recifes%20de%20coral">
    <rdfs:label>Zonas de recifes de coral</rdfs:label>
    <rdfs:comment>These are areas within a fringing reef where coral reefs are found.</rdfs:comment>
    <rdfs:subClassOf rdf:resource="#Recifes%20de%20coral"/>
  </owl:Class>
  <owl:Class rdf:about="#Recifes%20de%20coral">
    <rdfs:label>Recifes de coral</rdfs:label>
    <rdfs:comment>These are underwater ecosystems characterized by reef-building corals, providing a unique habitat for various marine species.</rdfs:comment>
    <rdfs:subClassOf rdf:resource="#ecossistemas%20costeiros%20brasileiros"/>
  </owl:Class>
  <owl:Class rdf:about="#Recifes%20de%20coral%20de%20barreira">
    <rdfs:label>Recifes de coral de barreira</rdfs:label>
    <rdfs:comment>These are similar to Recifes de barreira, long and continuous coral reef systems separated from the shore by a lagoon.</rdfs:comment>
    <rdfs:subClassOf rdf:resource="#Zonas%20de%20recifes%20de%20coral"/>
  </owl:Class>
  <owl:Class rdf:about="#Coral%20reef%20zones%20(fore%20reef">
    <rdfs:label>Coral reef zones (fore reef</rdfs:label>
    <rdfs:comment>Coral reef zones (fore reef is a subcategory of Zonas de recifes de coral. These are areas within a fringing reef where coral reefs are found.</rdfs:comment>
    <rdfs:subClassOf rdf:resource="#Zonas%20de%20recifes%20de%20coral"/>
  </owl:Class>
  <owl:Class rdf:about="#Estuários">
    <rdfs:label>Estuários</rdfs:label>
    <rdfs:comment>These are the tidal mouths of large rivers, where the tide meets the stream.</rdfs:comment>
    <rdfs:subClassOf rdf:resource="#ecossistemas%20costeiros%20brasileiros"/>
  </owl:Class>
  <owl:Class rdf:about="#ecossistemas%20costeiros%20brasileiros">
    <rdfs:label>ecossistemas costeiros brasileiros</rdfs:label>
    <rdfs:comment>"Ecossistemas costeiros brasileiros" is a Portuguese term that refers to the coastal ecosystems of Brazil. These are biological environments found along the Brazilian coastline, including a variety of habitats such as mangroves, sand dunes, lagoons, and coral reefs, which are home to diverse species of flora and fauna.</rdfs:comment>
  </owl:Class>
  <owl:Class rdf:about="#Zonas%20de%20frente%20de%20recife">
    <rdfs:label>Zonas de frente de recife</rdfs:label>
    <rdfs:comment>These are the areas of the reef that face towards the shore.</rdfs:comment>
    <rdfs:subClassOf rdf:resource="#Recifes%20de%20coral%20de%20barreira"/>
  </owl:Class>
  <owl:Class rdf:about="#Recifes%20de%20coral%20de%20franja">
    <rdfs:label>Recifes de coral de franja</rdfs:label>
    <rdfs:comment>These are similar to Recifes de franja, coral reefs attached directly to the shore.</rdfs:comment>
    <rdfs:subClassOf rdf:resource="#Zonas%20de%20recifes%20de%20coral"/>
  </owl:Class>
  <owl:Class rdf:about="#Zonas%20de%20recifes%20de%20barreira">
    <rdfs:label>Zonas de recifes de barreira</rdfs:label>
    <rdfs:comment>These are areas within a barrier reef where coral reefs are found.</rdfs:comment>
    <rdfs:subClassOf rdf:resource="#Recifes%20de%20coral%20de%20barreira"/>
  </owl:Class>
  <owl:Class rdf:about="#Biodiversidade%20de%20recifes%20de%20corais">
    <rdfs:label>Biodiversidade de recifes de corais</rdfs:label>
    <rdfs:comment>This refers to the biodiversity found in coral reefs.</rdfs:comment>
    <rdfs:subClassOf rdf:resource="#Recifes%20de%20coral%20de%20plataforma%20continental"/>
    <rdfs:subClassOf rdf:resource="#Zonas%20de%20recifes%20de%20barreira"/>
  </owl:Class>
  <owl:Class rdf:about="#Zonas%20de%20lagoa%20de%20recife">
    <rdfs:label>Zonas de lagoa de recife</rdfs:label>
    <rdfs:comment>These are the areas of the reef that are within the lagoon.</rdfs:comment>
    <rdfs:subClassOf rdf:resource="#Recifes%20de%20coral%20de%20barreira"/>
  </owl:Class>
  <owl:Class rdf:about="#Recifes%20de%20coral%20de%20plataforma%20continental">
    <rdfs:label>Recifes de coral de plataforma continental</rdfs:label>
    <rdfs:comment>These are reefs that grow on the continental shelf, in deeper waters.</rdfs:comment>
    <rdfs:subClassOf rdf:resource="#Zonas%20de%20recifes%20de%20plataforma"/>
  </owl:Class>
  <owl:Class rdf:about="#Colônias%20de%20corais">
    <rdfs:label>Colônias de corais</rdfs:label>
    <rdfs:comment>These are groups of coral polyps that live together on the reef, often of the same species.</rdfs:comment>
    <rdfs:subClassOf rdf:resource="#Coral%20reef%20zones%20(fore%20reef"/>
  </owl:Class>
</rdf:RDF>
